# $\S 2.3$ 高阶导数
## 定义
* $f'(x)$ 可导，有 $\displaystyle [f'(x)]'=\lim_{\Delta x\to 0}\dfrac{f'(x+\Delta x)-f'(x)}{\Delta x}$，则称$f(x)$**二阶可导**，记作 $f''(x)$ 、$y''$ 或 $\dfrac{\mathrm d^2y}{\mathrm dx^2}$。
> 类似地，有 $f'''(x)=\dfrac{\mathrm d^3y}{\mathrm dx^3}$ 或 $f^{(3)}(x)$， $f''''(x)=\dfrac{\mathrm d^4y}{\mathrm dx^4}$ 或 $f^{(4)}(x)$ ……$f^{(n)}(x)=\dfrac{\mathrm d^ny}{\mathrm dx^n}$

* 若 $f(x)$ 在 $(a,b)$ 内存在 $n$ 阶导数，且 $f^{(n)}(x)$ 在 $(a,b)$ 内连续，则$f(x)\in C^{(n)}(a,b)$

### 例题
1. $y=2x^2+e^x$，$y'=4x+e^x$，$y''=4+e^x$，$y'''=e^x$，……$y^{(n)}=e^x(n \ge 3)$
2. $y=P_n(x)=a_nx^n+a_{n-1}x^{n-1}+\cdots +a_1x+a_0$
	  * $y'=na_nx^{n-1}+(n-1)a_{n-1}x^{n-2}+\cdots+2a_2x+a_1+0$
	  * $y''=n(n-1)a_nx^{n-2}+\cdots+3\cdot 2a_3x+2a_2$
	  * $y^{(k)}=n(n-1)\cdots(n-k+1)a_nx^{n-k}+\cdots+(k+1)!a_{k+1}x+k!a_k(0\le k\le n)$
	  * $y^{(n)}=n!a_n$
	  * $y^{(k)}=0(k\gt n)$
3. 基本初等函数的高阶导数（常用）
	  * $y=C$，$y^{(n)}=0$
	  * $y=x^\mu$，$y^{(n)}=\mu(\mu-1)(\mu-2)\cdots(\mu-n+1)x^{\mu-n}$，$(x\ne 0)$
	  * $y=a^x$，$y^{(n)}=(\ln a)^na^x$，特别地，$(e^x)^{(n)}=e^x$
	  * $y=\log_a{x}$，$y^{(n)}=\dfrac{(-1)^{n-1}\cdot (n-1)!}{\ln a\cdot x^n}$，特别地，$(\ln x)^{(n)}=\dfrac{(-1)^{n-1}\cdot (n-1)!}{x^n}$
	  * $y=\sin x$，$y^{(n)}=\sin (x+n\cdot \dfrac{\pi}{2})$，$(\sin ax)^{(n)}=a^n\sin(ax+n\cdot \dfrac{\pi}{2})$
	  * $y=\cos x$，$y^{(n)}=\cos (x+n\cdot \dfrac{\pi}{2})$，$(\cos ax)^{(n)}=a^n\cos(ax+n\cdot \dfrac{\pi}{2})$

## 高阶求导运算法则
1. $u(x)$，$v(x)$ 均为 $n$ 阶可导
$$
	[u(x)\pm v(x)]^{(n)}=u^{(n)}(x)+v^{(n)}(x)
$$
2. $[Cu(x)]^{(n)}=Cu^{(n)}(x)$，$C$ 为常数
3. (Leibniz公式)
$$
  [u(x)v(x)]^{(n)}=C_n^0u^{(n)}v+C_n^1u^{(n-1)}v'+\cdots +C_n^nuv^{(n)}
$$

### 例题
1. $y=x^2\cdot e^{2x}$，求$y^{(n)}$

解：
$$
  y^{(n)}=(x^2e^{2x})^{(n)}=C_n^0(e^{2x})^{(n)}x^2+C_n^1(e^{2x})^{(n-1)}\cdot 2x+C_n^2(e^{2x})^{(n-2)}\cdot 2 +0+\cdots +0 \\
	(e^{2x})^{(n)}=2^ne^{2x} \\
	原式=e^{2x}(x^22^n+xn2^n+n(n-1)2^{n-2})
$$
2. $y=\dfrac{1}{1-x^2}$，求$y^{(n)}$

解：

$y=\dfrac{1}{1+x}\cdot \dfrac{1}{1-x}$

$(\dfrac{1}{1-x})^{(n)}=n!(1-x)^{-1-n}$

$(\dfrac{1}{1+x})^{(n)}=[(-1)(1+x)^{-2}]^{(n-1)}=[(-1)(-2)(1+x)^{-3}]^{(n-2)}=(-1)^nn!(1+x)^{-1-n}$

$y^{(n)}=\left(\dfrac{1}{1+x}\cdot \dfrac{1}{1-x}\right)^{(n)}=C_n^0n!(1-x)^{-1-n}\cdot \dfrac{1}{1+x}+C_n^1(n-1)!(1-x)^{-1+n+1}+\cdots +C_n^n\dfrac{1}{1+x}\cdot n!(1-x)^{-1-n}$

3. $y=\arctan x$，求$y^{(n)}(0)$

解：

$y'=\dfrac{1}{1+x^2} \quad y'(0)=1$

$y''=-\dfrac{2x}{(1+x^2)^2} \quad y''(0)=0$

$y'''=-2\left[1\cdot \dfrac{1}{(1+x^2)^2}+x\cdot \left(\dfrac{1}{(1+x^2)^2}\right)'\right] \quad y'''(0)=-2$

$y'(1+x^2)=1$，两边关于 $x$ 求 $n$ 阶导

$C_n^0(y')^{(n)}(1+x^2)+C_n^1(y')^{(n-1)}\cdot 2x+C_n^2(y')^{(n-2)}\cdot 2=0$

当 $x=0$ 时，$y^{(n+1)}(0)(1+0^2)+\dfrac{n(n-1)}{2!}y^{(n-1)}(0)\cdot 2=0$

$\because y(0)=0,y'(0)=1,y''(0)=0$

$\therefore y^{(n+1)}(0)=-n(n-1)y^{(n-1)}(0)$ 得

$$
\begin{cases}
y^{(2k)}(0)&=0\\
y^{(2k+1)}(0)&=(-1)^k(2k)!
\end{cases}，其中k=0,1,2,\cdots
$$

4. $g'(x)$ 连续，且 $f(x)=(x-a)^2g(x)$，求$f''(a)$

解：

$$
\begin{align*}
f''(a)&=\lim_{x\to a}\dfrac{f'(x)-f'(a)}{x-a}\\
&=\lim_{x\to a}\dfrac{2(x-a)g(x)+(x-a)^2g'(x)}{x-a}\\
&=\lim_{x\to a}[2g(x)+(x-a)g'(x)]
\end{align*}
$$

且 $f'(x)|_{x=a}=0$

$\therefore g'(x)$ 连续 $\displaystyle \Rightarrow \lim_{x\to a}g'(x)=g'(a) \Rightarrow g(x)$ 连续 $\displaystyle \Rightarrow \lim_{x\to a}g(x)=g(a)$

$\therefore f''(a)=2g(a)+0=2g(a)$

5. $\dfrac{\mathrm{d}x}{\mathrm{d}y}=\dfrac{1}{y'}$，求证 $\dfrac{\mathrm{d}^2x}{\mathrm{d}y^2}=-\dfrac{y''}{(y')^3}$

证：

$\dfrac{\mathrm{d}x}{\mathrm{d}y}=\dfrac{\mathrm{d}}{\mathrm{d}y}\left(\dfrac{1}{y'}\right)=(-1)\dfrac{1}{(y')^2}\cdot \left(\dfrac{\mathrm{d}}{\mathrm{d}y} y'\right)=-\dfrac{1}{(y')^2}\cdot (y''\cdot \dfrac{1}{y'})=-\dfrac{y''}{(y')^3}$
